SLL_optimization_sound.v
@@ -1,8 +1,337 @@
-Require Import SLLPrediction.
+Require Import List.
+Require Import GallStar.SLLPrediction.
+Require Import GallStar.Tactics.
+Import ListNotations.
 
 Module SllOptimizationSoundFn (Import D : Defs.T).
 
   Module Export SLLP := SllPredictionFn D.
+
+  (* Definitions to capture the fact that SLL prediction overapproximates 
+     LL prediction. For each LL subparser in play, there exists a corresponding
+     SLL subparser that carries the same prediction and has a stack that matches
+     the stack top of the LL subparser. There might also be SLL subparsers in 
+     play that don't correspond to any of the LL subparsers, but prediction will
+     fail over to LL mode if SLL mode finds more than one viable right-hand side.
+     That's why SLL prediction is a _sound_ overapproximation of LL prediction. *)
+  Definition approx (sp' sp : subparser) : Prop :=
+    match sp', sp with
+    | Sp pred' (fr', frs'), Sp pred (fr, frs) =>
+      pred' = pred
+      /\ exists ctx, fr' :: frs' ++ ctx = fr :: frs
+    end.
+
+  Definition overapprox (sps' sps : list subparser) : Prop :=
+    forall sp, In sp sps -> exists sp', In sp' sps' /\ approx sp' sp.
+
+  (*
+  (* need some more invariants here *)
+  Lemma sllPredict'_overapprox_llPredict' :
+    forall g cm ts sps' sps ca ca' sll_res ll_res,
+      cache_stores_target_results g cm ca
+      -> overapprox sps' sps
+      -> sllPredict' g cm sps' ts ca = (sll_res, ca')
+      -> llPredict' g sps ts = ll_res
+      -> match sll_res with
+         | PredAmbig ys => True
+         | PredSucc ys  =>
+           ll_res = PredSucc ys \/ ll_res = PredReject
+         | PredReject =>
+           ll_res = PredReject
+         | PredError e =>
+           True
+         end.
+  Proof.
+    intros g cm ts; induction ts as [| (a,l) ts IH]; intros sps' sps ca ca' sll_res ll_res hc ho hs hl; sis.
+    - (* no more tokens left *)
+      destruct sps as [| sp sps]; subst.
+      + destruct sps' as [| sp' sps'].
+        * inv hs; auto.
+        * destruct (allPredictionsEqual sp' sps') eqn:ha'; inv hs; auto.
+          dm; auto.
+      + destruct sps' as [| sp' sps'].
+        * (* overapprox contra *)
+          admit.
+        * destruct (allPredictionsEqual sp' sps') eqn:ha'; inv hs; auto.
+          -- assert (Hass : allPredictionsEqual sp sps = true) by admit.
+          rewrite Hass.
+          admit.
+          -- dmeq hh; auto.
+             ++ unfold handleFinalSubparsers in hh. dmeqs H; tc; auto.
+                ** inv hh.
+          assert (
+          -- inv hs; auto.
+          -- 
+      + destruct 
+        * inv hs.
+          
+      destruct sps' as [| sp' sps']; destruct sps as [| sp sps]; inv hs; auto.
+            destruct sps as [| sp sps]; auto.
+      destruct (allPredictionsEqual sp' sps') eqn:ha.
+      + (* overapprox + SLL allPredictionsEqual = LL allPredictionsEqual *)
+        inv hs.
+        assert (Hass : allPredictionsEqual sp sps = true) by admit.
+        simpl. rewrite Hass.
+        admit.
+      + inv hs. rename H0 into hh.
+        unfold handleFinalSubparsers in *.
+        (* handleFinalSubparsers will extract the sps in final
+           configurations, and the resulting ones will have
+           allPredictionsEqual = true, so allPredictionsEqual
+           will also be true for the LL subparsers in final 
+           configurations *)
+        admit.
+    - (* there's a head token left *)
+      destruct sps  as [| sp sps]; auto.
+      destruct sps' as [| sp' sps']; tc.
+      destruct (allPredictionsEqual sp' sps') eqn:ha'.
+      + inv hs.
+        assert (Hass : allPredictionsEqual sp sps = true) by admit.
+        simpl. rewrite Hass.
+        (* same as the case above *)
+        admit.
+      + destruct (allPredictionsEqual sp sps) eqn:ha in hl.
+        * (* tricky case: LL prediction has converged on a 
+             prediction, but SLL prediction hasn't *)
+          (* maybe we can prove that if llPredict' returns 
+             PredSucc ys when there's a token left, then 
+             llPredict' on the tail returns either the same prediction 
+             or reject *)
+          destruct (Cache.find _ _) as [sps''' |] eqn:hf.
+          -- apply hc in hf.
+             subst. left.
+             
+             assert (Hass : exists sps'' ll_r,
+                        llPredict' g sps'' ts = ll_r
+                        /\ (ll_r = PredSucc (prediction sp)
+                            \/ ll_r = PredReject)) by admit.
+             destruct Hass as [sps'' [ll_r' [ heq htail]]].
+             eapply IH with (sps := sps'')
+                            (ll_r := ll_r') in hs; eauto.
+             ++ destruct hs; destruct htail; subst.
+                ** inv H0; auto.
+                ** inv H0.
+                ** inv H0.
+                ** right. rewrite <- hl'. rewrite <- heq.
+             ++ 
+             destruct htail as [hsuc | hrej].
+             ++ subst.
+                eapply IH with (sps := sps'') in hs; eauto.
+                (* overapprox invariant is preserved *)
+                admit.
+             ++ eapply IH with (sps := sps'')
+                               (ll_r := ll_r') in hs; eauto.
+                ** subst.
+                   left.
+                   admit.
+                ** admit.
+          -- 
+                ** subst.
+                eapp
+                (ll_r := ll_r') in hs; eauto.
+             clear hl. clear hl'.
+
+             ++ eapply IH with (sps  := sps''); eauto.
+                               (ll_r := PredSucc (prediction sp)) in hs; eauto.
+                ** admit.
+                ** 
+          assert (Hass : exists sps'', llPredict' g sps'' ts =
+                                       PredSucc (prediction sp) \/ llPredict' g sps'' ts = PredReject) by admit.
+          destruct Hass as [sps'' htail].
+          destruct (Cache.find _ _) as [sps''' |] eqn:hf.
+          -- apply hc in hf.
+             destruct htail.
+             ++ eapply IH with (sps := sps'') in hs; eauto.
+                ** (* invariant preserved *)
+                  admit.
+                ** subst; auto.
+             ++ eapply IH with (sps := sps'') (ll_r := PredReject) in hs; eauto.
+                ** subst; auto.
+        * eapply IH in hs; eauto.
+        inv hs.
+inv hs.
+
+    
+         | ll_r = PredSucc ys \/ ll_r = PredReject.
+  Proof.
+   *)
+
+  (* to do : maybe I should redefine llPredict'
+     and sllPredict' so that they call handleFinalSubparsers
+     right away when the remaining token list is empty *)
+  (* need some more invariants here *)
+  Lemma sllPredict'_succ_llPredict'_succ_or_reject :
+    forall g cm ts sps' sps ca ys ca' ll_r,
+      cache_stores_target_results g cm ca
+      -> overapprox sps' sps
+      -> sllPredict' g cm sps' ts ca = (PredSucc ys, ca')
+      -> llPredict' g sps ts = ll_r
+      -> ll_r = PredSucc ys \/ ll_r = PredReject.
+  Proof.
+    intros g cm ts; induction ts as [| (a,l) ts IH]; intros sps' sps ca ys ca' ll_r hc ho hs hl; simpl in hs; pose proof hl as hl'; simpl in hl.
+    - (* no more tokens left *)
+      destruct sps as [| sp sps]; auto.
+      destruct sps' as [| sp' sps']; tc.
+      destruct (allPredictionsEqual sp' sps') eqn:ha.
+      + (* overapprox + SLL allPredictionsEqual = LL allPredictionsEqual *)
+        inv hs.
+        assert (Hass : allPredictionsEqual sp sps = true) by admit.
+        simpl. rewrite Hass.
+        admit.
+      + inv hs. rename H0 into hh.
+        unfold handleFinalSubparsers in *.
+        (* handleFinalSubparsers will extract the sps in final
+           configurations, and the resulting ones will have
+           allPredictionsEqual = true, so allPredictionsEqual
+           will also be true for the LL subparsers in final 
+           configurations *)
+        destruct (allPredictionsEqual sp sps) eqn:ha'.
+        * dmeqs H; tc. inv hh.
+        admit.
+    - (* there's a head token left *)
+      destruct sps  as [| sp sps]; auto.
+      destruct sps' as [| sp' sps']; tc.
+      destruct (allPredictionsEqual sp' sps') eqn:ha'.
+      + inv hs.
+        assert (Hass : allPredictionsEqual sp sps = true) by admit.
+        simpl. rewrite Hass.
+        (* same as the case above *)
+        admit.
+      + destruct (allPredictionsEqual sp sps) eqn:ha in hl.
+        * (* tricky case: LL prediction has converged on a 
+             prediction, but SLL prediction hasn't *)
+          (* maybe we can prove that if llPredict' returns 
+             PredSucc ys when there's a token left, then 
+             llPredict' on the tail returns either the same prediction 
+             or reject *)
+          destruct (Cache.find _ _) as [sps''' |] eqn:hf.
+          -- apply hc in hf.
+             subst. left.
+             
+             assert (Hass : exists sps'' ll_r,
+                        llPredict' g sps'' ts = ll_r
+                        /\ (ll_r = PredSucc (prediction sp)
+                            \/ ll_r = PredReject)) by admit.
+             destruct Hass as [sps'' [ll_r' [ heq htail]]].
+             eapply IH with (sps := sps'')
+                            (ll_r := ll_r') in hs; eauto.
+             ++ destruct hs; destruct htail; subst.
+                ** inv H0; auto.
+                ** inv H0.
+                ** inv H0.
+                ** right. rewrite <- hl'. rewrite <- heq.
+             ++ 
+             destruct htail as [hsuc | hrej].
+             ++ subst.
+                eapply IH with (sps := sps'') in hs; eauto.
+                (* overapprox invariant is preserved *)
+                admit.
+             ++ eapply IH with (sps := sps'')
+                               (ll_r := ll_r') in hs; eauto.
+                ** subst.
+                   left.
+                   admit.
+                ** admit.
+          -- 
+                ** subst.
+                eapp
+                (ll_r := ll_r') in hs; eauto.
+             clear hl. clear hl'.
+
+             ++ eapply IH with (sps  := sps''); eauto.
+                               (ll_r := PredSucc (prediction sp)) in hs; eauto.
+                ** admit.
+                ** 
+          assert (Hass : exists sps'', llPredict' g sps'' ts =
+                                       PredSucc (prediction sp) \/ llPredict' g sps'' ts = PredReject) by admit.
+          destruct Hass as [sps'' htail].
+          destruct (Cache.find _ _) as [sps''' |] eqn:hf.
+          -- apply hc in hf.
+             destruct htail.
+             ++ eapply IH with (sps := sps'') in hs; eauto.
+                ** (* invariant preserved *)
+                  admit.
+                ** subst; auto.
+             ++ eapply IH with (sps := sps'') (ll_r := PredReject) in hs; eauto.
+                ** subst; auto.
+        * eapply IH in hs; eauto.
+        inv hs.
+inv hs.
+        
+  Admitted.
+
+  
+  (* need some more invariants here *)
+  Lemma sllPredict'_succ_llPredict'_succ_or_reject :
+    forall g cm ts sps' sps ca ys ca',
+      overapprox sps' sps
+      -> sllPredict' g cm sps' ts ca = (PredSucc ys, ca')
+      -> llPredict' g sps ts = PredSucc ys
+         \/ llPredict' g sps ts = PredReject.
+  Proof.
+    intros g cm ts; induction ts as [| (a,l) ts IH]; intros sps' sps ca ys ca' ho hs; simpl in hs.
+    - (* no more tokens left *)
+      destruct sps as [| sp sps]; auto.
+      destruct sps' as [| sp' sps']; tc.
+      destruct (allPredictionsEqual _ _) eqn:ha.
+      + (* overapprox + SLL allPredictionsEqual = LL allPredictionsEqual *)
+        inv hs.
+        assert (Hass : allPredictionsEqual sp sps = true) by admit.
+        simpl. rewrite Hass.
+        admit.
+      + inv hs. rename H0 into hh.
+        unfold handleFinalSubparsers in *.
+        (* handleFinalSubparsers will extract the sps in final
+           configurations, and the resulting ones will have
+           allPredictionsEqual = true, so allPredictionsEqual
+           will also be true for the LL subparsers in final 
+           configurations *)
+        admit.
+    - (* there's a head token left *)
+      destruct sps as [| sp sps]; auto.
+      destruct sps' as [| sp' sps']; tc.
+      destruct (allPredictionsEqual sp' sps') eqn:ha'.
+      + inv hs.
+        assert (Hass : allPredictionsEqual sp sps = true) by admit.
+        simpl. rewrite Hass.
+        (* same as the case above *)
+        admit.
+      + simpl. subst.
+        destruct (allPredictionsEqual sp sps) eqn:ha.
+        * (* tricky case: LL prediction has converged on a 
+             prediction, but SLL prediction hasn't *)
+        destruct (Cache.find _ _) as [sps'' |] eqn:hf.
+        * eapply IH in hs; eauto.
+        inv hs.
+inv hs.
+        
+  Admitted.
+
+  Lemma sllPredict_succ_llPredict_succ_or_reject :
+    forall g cm ss o x suf frs ts ca ys ca',
+      ss = (SF o (NT x :: suf), frs)
+      -> no_left_recursion g
+      -> suffix_stack_wf g ss
+      -> sllPredict g cm x ts ca = (PredSucc ys, ca')
+      -> llPredict g x ss ts  = PredSucc ys
+         \/ llPredict g x ss ts  = PredReject.
+  Proof.
+    intros g cm ss o x suf frs ts ca ys ca' ? hn hw hp; subst.
+    unfold llPredict; unfold sllPredict in hp; dmeqs H; tc; inv hp.
+    - exfalso; eapply startState_never_returns_error; eauto.
+    - eapply sllPredict'_succ_llPredict'_succ_or_reject; eauto.
+  Qed.
+  
+  Lemma adaptivePredict_succ_llPredict_succ_or_reject :
+    forall g cm x ss ts ca ys ca',
+      adaptivePredict g cm x ss ts ca = (PredSucc ys, ca')
+      -> llPredict g x ss ts = PredSucc ys
+         \/ llPredict g x ss ts = PredReject.
+  Proof.
+    intros g cm x ss ts ca ys ca' hp.
+    unfold adaptivePredict in hp; dmeqs H; tc; inv hp; auto.
+    eapply sllPredict_succ_llPredict_succ_or_reject; eauto.
+  Qed.
 
 End SllOptimizationSoundFn.
 
